Move some codes to test/.

Dijkstra.lean
@@ -5,42 +5,10 @@ Released under Apache 2.0 license as described in the file LICENSE.
 
 import Dijkstra.Init
 import Dijkstra.Control.Lawful
+import Dijkstra.Control.Functor.Subreg
 import Dijkstra.Control.Monad.Hom
 import Dijkstra.Control.Monad.Rel
 import Dijkstra.Control.Monad.Dijkstra
+import Dijkstra.Control.Monad.Reify
 import Dijkstra.Control.Monad.Spec
 import Dijkstra.Control.Monad.Transformer
-
-universe u
-
-@[reducible]
-def WPExcept (ε : Type u) := ExceptT ε WPPure
-
-instance (ε : Type u) : Monad (WPExcept ε) :=
-  inferInstanceAs (Monad (ExceptT ε WPPure))
-
-protected
-def WPExcept.rel (ε : Type u) : MonadRel (WPExcept ε) (WPExcept ε) where
-  rel {α} x y := ∀ (p : Except ε α → Prop), y.predT p → x.predT p
-  pure a p := by dsimp; exact id
-  bind {α} {β} {x} {y} f g hxy hfg p := by
-    dsimp [bind] at *
-    dsimp [ExceptT.bind, ExceptT.mk]
-    apply mrel_bind (m:=WPPure) hxy
-    intro a
-    cases a
-    case a.error e =>
-      dsimp [ExceptT.bindCont]
-      exact mrel_pure (m:=WPPure) _
-    case a.ok a =>
-      dsimp [ExceptT.bindCont]
-      exact hfg a
-
-instance (ε : Type u) : SpecMonad (WPExcept ε) where
-  rel := WPExcept.rel ε
-  trans := by
-    dsimp [WPExcept.rel]
-    intro α x y z hxy hyz p hp
-    exact hxy p (hyz p hp)
-
-example (ε : Type u) (α : Type _) : WPPure α → WPExcept ε α := monadLift
