test/WPExcept.lean
@@ -1,0 +1,40 @@
+/-
+Copyright (c) 2022 Jun Yoshida. All rights reserved.
+Released under Apache 2.0 license as described in the file LICENSE.
+-/
+
+import Dijkstra
+
+universe u
+
+@[reducible]
+def WPExcept (ε : Type u) := ExceptT ε WPPure
+
+instance (ε : Type u) : Monad (WPExcept ε) :=
+  inferInstanceAs (Monad (ExceptT ε WPPure))
+
+protected
+def WPExcept.rel (ε : Type u) : MonadRel (WPExcept ε) (WPExcept ε) where
+  rel {α} x y := ∀ (p : Except ε α → Prop), y.predT p → x.predT p
+  pure a p := by dsimp; exact id
+  bind {α} {β} {x} {y} f g hxy hfg p := by
+    dsimp [bind] at *
+    dsimp [ExceptT.bind, ExceptT.mk]
+    apply mrel_bind (m:=WPPure) hxy
+    intro a
+    cases a
+    case a.error e =>
+      dsimp [ExceptT.bindCont]
+      exact mrel_pure (m:=WPPure) _
+    case a.ok a =>
+      dsimp [ExceptT.bindCont]
+      exact hfg a
+
+instance (ε : Type u) : SpecMonad (WPExcept ε) where
+  rel := WPExcept.rel ε
+  trans := by
+    dsimp [WPExcept.rel]
+    intro α x y z hxy hyz p hp
+    exact hxy p (hyz p hp)
+
+example (ε : Type u) (α : Type _) : WPPure α → WPExcept ε α := monadLift
